Weidenbach_Book/IsaSAT_Decide.thy
@@ -1,5 +1,5 @@
 theory IsaSAT_Decide
-  imports IsaSAT_Setup IsaSAT_VMTF
+  imports IsaSAT_Setup IsaSAT_VMTF IsaSAT_Rephase
 begin
 
 
@@ -393,9 +393,19 @@ where
       None \<Rightarrow> RETURN (True, S)
     | Some L \<Rightarrow> do {
         T \<leftarrow> decide_lit_wl_heur L S;
+        T \<leftarrow> save_phase_st T;
         RETURN (False, T)}
   })
 \<close>
+
+
+lemma save_phase_st_spec:
+  \<open>(S, S') \<in> twl_st_heur''' r \<Longrightarrow> save_phase_st S \<le> SPEC(\<lambda>S. (S, S') \<in> twl_st_heur''' r)\<close>
+  unfolding save_phase_st_def
+  apply (cases S')
+  apply (refine_vcg save_phase_heur_spec[THEN order_trans, of \<open>all_atms_st S'\<close>])
+  apply (simp_all add:  twl_st_heur_def)
+  done
 
 lemma decide_wl_or_skip_D_heur_decide_wl_or_skip_D:
   \<open>(decide_wl_or_skip_D_heur, decide_wl_or_skip) \<in> twl_st_heur''' r \<rightarrow>\<^sub>f \<langle>bool_rel \<times>\<^sub>f twl_st_heur''' r\<rangle> nres_rel\<close>
@@ -409,7 +419,8 @@ proof -
 
   have final: \<open>decide_lit_wl_heur xb x1a
 	\<le> SPEC
-	   (\<lambda>T. RETURN (False, T)
+	   (\<lambda>T.  do {T \<leftarrow> save_phase_st T;
+                  RETURN (False, T)}
 		\<le> SPEC
 		   (\<lambda>c. (c, False, decide_lit_wl x'a x1)
 			\<in> bool_rel \<times>\<^sub>f twl_st_heur''' r))\<close>
@@ -433,7 +444,7 @@ proof -
   proof -
     show ?thesis
       unfolding decide_lit_wl_heur_def
-        decide_lit_wl_def
+        decide_lit_wl_def save_phase_st_def
       apply (cases x1a)
       apply refine_vcg
       subgoal
@@ -443,21 +454,36 @@ proof -
         by (rule cons_trail_Decided_tr_pre[of _ \<open>get_trail_wl x1\<close> \<open>all_atms_st x1\<close>])
 	  (use that(2) in \<open>auto simp: twl_st_heur_def st all_atms_def[symmetric]\<close>)
       subgoal
-        using that(2) unfolding cons_trail_Decided_def[symmetric] st
-        by (auto simp add: twl_st_heur_def all_atms_def[symmetric]
+        using that(2) unfolding cons_trail_Decided_def[symmetric] st apply -
+        apply (rule  save_phase_heur_spec[THEN order_trans, of \<open>all_atms_st x1\<close>])
+        apply (auto simp: twl_st_heur_def)[]
+        apply (clarsimp simp add: twl_st_heur_def all_atms_def[symmetric] 
+	   isa_length_trail_length_u[THEN fref_to_Down_unRET_Id] out_learned_def
+	  intro!: cons_trail_Decided_tr[THEN fref_to_Down_unRET_uncurry]
+	    isa_vmtf_consD2)
+        by (auto simp add: twl_st_heur_def all_atms_def[symmetric] 
 	   isa_length_trail_length_u[THEN fref_to_Down_unRET_Id] out_learned_def
 	  intro!: cons_trail_Decided_tr[THEN fref_to_Down_unRET_uncurry]
 	    isa_vmtf_consD2)
       done
   qed
 
+  have decide_wl_or_skip_alt_def: \<open>decide_wl_or_skip S = (do {
+    ASSERT(decide_wl_or_skip_pre S);
+    (S, L) \<leftarrow> find_unassigned_lit_wl S;
+    case L of
+      None \<Rightarrow> RETURN (True, S)
+    | Some L \<Rightarrow> RETURN (False, decide_lit_wl L S)
+  })\<close> for S
+  unfolding decide_wl_or_skip_def by auto
   show ?thesis
     supply [[goals_limit=1]]
-    unfolding decide_wl_or_skip_D_heur_def decide_wl_or_skip_def decide_wl_or_skip_pre_def
+    unfolding decide_wl_or_skip_D_heur_def decide_wl_or_skip_alt_def decide_wl_or_skip_pre_def
      decide_l_or_skip_pre_def twl_st_of_wl.simps[symmetric]
     apply (intro nres_relI frefI same_in_Id_option_rel)
-    apply (refine_vcg find_unassigned_lit_wl_D'_find_unassigned_lit_wl_D[of r, THEN fref_to_Down])
-    subgoal
+    apply (refine_vcg find_unassigned_lit_wl_D'_find_unassigned_lit_wl_D[of r, THEN fref_to_Down]
+      save_phase_st_spec[of _ _ r])
+    subgoal for x y
       unfolding decide_wl_or_skip_pre_def find_unassigned_lit_wl_D_heur_pre_def
 	decide_wl_or_skip_pre_def decide_l_or_skip_pre_def decide_or_skip_pre_def
        apply normalize_goal+
@@ -468,23 +494,10 @@ proof -
     apply (rule same_in_Id_option_rel)
     subgoal by (auto simp del: simp: twl_st_heur_def)
     subgoal by (auto simp del: simp: twl_st_heur_def)
-    apply (rule final; assumption)
+    apply (rule final; assumption?)
     done
  qed
 
-
-term \<open>do {
-      ((M, vm), L) \<leftarrow> isa_vmtf_find_next_undef_upd M vm;
-      ASSERT(L \<noteq> None \<longrightarrow> get_saved_phase_heur_pre (the L) heur);
-      case L of 
-       None \<Rightarrow> RETURN (True, bb)
-     | Some L \<Rightarrow> do {
-        b \<leftarrow> mop_get_saved_phase_heur L heur;
-        L \<leftarrow> RETURN (if b then Pos L else Neg L);
-        T \<leftarrow> decide_lit_wl_heur L' aa;
-        RETURN (False, T)
-      }
-      }\<close>
 
 lemma bind_triple_unfold:
   \<open>do {
@@ -510,6 +523,7 @@ definition decide_wl_or_skip_D_heur' where
         let L = (if b then Pos L else Neg L);
         T \<leftarrow> decide_lit_wl_heur L (M, N', D', j, W', vm, clvls, cach, lbd, outl, stats, heur,
           vdom, avdom, lcount, opts, old_arena);
+        T \<leftarrow> save_phase_st T;
         RETURN (False, T)
       }
     })
@@ -528,7 +542,7 @@ proof -
     apply (cases S, simp only:)
     unfolding decide_wl_or_skip_D_heur_def find_unassigned_lit_wl_D_heur_def
       nres_monad3 prod.case decide_wl_or_skip_D_heur'_def
-    apply (subst (3) bind_triple_unfold[symmetric])
+    apply (subst (4) bind_triple_unfold[symmetric])
     unfolding decide_wl_or_skip_D_heur_def find_unassigned_lit_wl_D_heur_def
       nres_monad3 prod.case lit_of_found_atm_def mop_get_saved_phase_heur_def
     apply refine_vcg
